proof/crefine/ARM_HYP/ADT_C.thy
@@ -659,8 +659,8 @@ lemma tcb_queue_rel'_unique:
 
 definition tcb_queue_C_to_tcb_queue :: "tcb_queue_C \<Rightarrow> tcb_queue" where
   "tcb_queue_C_to_tcb_queue q \<equiv>
-     TcbQueue (if head_C q = NULL then None else Some (ctcb_ptr_to_tcb_ptr (head_C q)))
-              (if end_C q = NULL then None else Some (ctcb_ptr_to_tcb_ptr (end_C q)))"
+     HeadEndPtrs (if head_C q = NULL then None else Some (ctcb_ptr_to_tcb_ptr (head_C q)))
+                 (if end_C q = NULL then None else Some (ctcb_ptr_to_tcb_ptr (end_C q)))"
 
 definition cready_queues_to_H ::
   "tcb_queue_C[num_tcb_queues] \<Rightarrow> (domain \<times> priority \<Rightarrow> ready_queue)"
@@ -670,7 +670,7 @@ definition cready_queues_to_H ::
        if qdom \<le> maxDomain \<and> prio \<le> maxPriority
        then let cqueue = index cs (cready_queues_index_to_C qdom prio)
              in tcb_queue_C_to_tcb_queue cqueue
-       else TcbQueue None None"
+       else emptyQueue"
 
 lemma cready_queues_to_H_correct:
   "\<lbrakk>cready_queues_relation (ksReadyQueues s) (ksReadyQueues_' ch);
@@ -687,20 +687,23 @@ lemma cready_queues_to_H_correct:
   apply clarsimp
   apply (frule (3) obj_at'_tcbQueueHead_ksReadyQueues)
   apply (frule (3) obj_at'_tcbQueueEnd_ksReadyQueues)
-  apply (frule tcbQueueHead_iff_tcbQueueEnd)
+  apply (frule he_ptrs_head_iff_he_ptrs_end)
   apply (rule conjI)
    apply (clarsimp simp: tcb_queue_C_to_tcb_queue_def ctcb_queue_relation_def option_to_ctcb_ptr_def)
    apply (case_tac "tcbQueueHead (ksReadyQueues s (d, p)) = None")
-    apply (clarsimp simp: tcb_queue.expand)
+    apply (clarsimp simp: headEndPtrsEmpty_def)
+    apply (metis head_end_ptrs.exhaust_sel)
    apply clarsimp
    apply (rename_tac queue_head queue_end)
    apply (prop_tac "tcb_at' queue_head s", fastforce simp: tcbQueueEmpty_def obj_at'_def)
    apply (prop_tac "tcb_at' queue_end s", fastforce simp: tcbQueueEmpty_def obj_at'_def)
    apply (drule kernel.tcb_at_not_NULL)+
-   apply (fastforce simp: tcb_queue.expand kernel.ctcb_ptr_to_ctcb_ptr)
-  apply (clarsimp simp: tcbQueueEmpty_def ctcb_queue_relation_def option_to_ctcb_ptr_def
+   apply (clarsimp simp: kernel.ctcb_ptr_to_ctcb_ptr)
+   apply (metis head_end_ptrs.exhaust_sel)
+  apply (clarsimp simp: emptyHeadEndPtrs_def tcbQueueEmpty_def
+                        ctcb_queue_relation_def option_to_ctcb_ptr_def
                  split: option.splits;
-         metis tcb_queue.exhaust_sel word_not_le)
+         metis head_end_ptrs.exhaust_sel word_not_le)
   done
 
 (* showing that cpspace_relation is actually unique >>>*)
